Code from SB course to make #155 reproducible again

examples/data_structures/binary_search_tree_basic.fst
@@ -7,17 +7,16 @@ type tree =
 val in_tree : int -> tree -> Tot bool
 let rec in_tree x t =
   match t with
-  | Leaf n -> false
+  | Leaf -> false
   | Node n t1 t2 -> x = n || in_tree x t1 || in_tree x t2
 
 val all : p:(int -> Tot bool) -> t:tree ->
             Tot (r:bool{r <==> (forall x. in_tree x t ==> p x)})
 let rec all p t =
   match t with
-  | Leaf n -> true
+  | Leaf -> true
   | Node n t1 t2 -> p n && all p t1 && all p t2
 
-(* CH: don't these already have some non-operator form? *)
 val lt : int -> int -> Tot bool
 let lt n1 n2 = n1 < n2
 
@@ -27,16 +26,26 @@ let gt n1 n2 = n1 > n2
 val is_bst : tree -> Tot bool
 let rec is_bst t =
   match t with
-  | Leaf n -> true
+  | Leaf -> true
   | Node n t1 t2 -> all (gt n) t1 && all (lt n) t2 && is_bst t1 && is_bst t2
 
 val search : x:int -> t:tree{is_bst t} -> Tot (r:bool{r <==> in_tree x t})
 let rec search x t =
   match t with
-  | Leaf n -> false
+  | Leaf -> false
   | Node n t1 t2 -> if x = n then      true
                     else if x < n then search x t1
                     else               search x t2
+
+val insert : x:int -> t:tree{is_bst t} ->
+             Tot (r:tree{is_bst r /\
+                  (forall y. in_tree y r <==> (in_tree y t \/ x = y))})
+let rec insert x t =
+  match t with
+  | Leaf -> Node x Leaf Leaf
+  | Node n t1 t2 -> if x = n then      t
+                    else if x < n then Node n (insert x t1) t2
+                    else               Node n t1 (insert x t2)
 
 (* This variant should also work, filed as #155
 val insert : x:int -> t:tree -> Pure tree
@@ -54,12 +63,72 @@ let rec insert x t =
                       admit()(*Node n t1 (insert x t2)*)
 *)
 
-val insert : x:int -> t:tree{is_bst t} ->
-             Tot (r:tree{is_bst r /\
-                  (forall y. in_tree y r <==> (in_tree y t \/ x = y))})
-let rec insert x t =
+val insert' : int -> tree -> Tot tree
+let rec insert' x t =
   match t with
   | Leaf -> Node x Leaf Leaf
   | Node n t1 t2 -> if x = n then      t
-                    else if x < n then Node n (insert x t1) t2
-                    else               Node n t1 (insert x t2)
+                    else if x < n then Node n (insert' x t1) t2
+                    else               Node n t1 (insert' x t2)
+
+val insert_lemma : x:int -> t:tree{is_bst t} -> Lemma
+      (is_bst (insert' x t) /\
+      (forall y. in_tree y (insert' x t) <==> in_tree y t \/ x = y))
+let rec insert_lemma x t = match t with
+  | Leaf -> ()
+  | Node _ t1 t2 -> insert_lemma x t1; insert_lemma x t2
+
+val ge : int -> int -> Tot bool
+let ge n1 n2 = n1 >= n2
+
+val find_max : t:tree{is_bst t /\ is_Node t} ->
+      Tot (x:int{all (ge x) t /\ in_tree x t})
+let rec find_max (Node n _ t2) = if is_Leaf t2 then n else find_max t2
+
+val find_max' : t:tree{is_Node t}-> Tot int
+let rec find_max' (Node n _ t2) = if is_Leaf t2 then n else find_max' t2
+
+val find_max_lemma : t:tree{is_Node t /\ is_bst t} ->
+      Lemma (in_tree (find_max' t) t /\ all (ge (find_max' t)) t)
+let rec find_max_lemma (Node _ _ t2) = if is_Node t2 then find_max_lemma t2
+
+val find_max_eq : t:tree{is_Node t /\ is_bst t} -> Lemma (find_max t = find_max' t)
+let find_max_eq t = find_max_lemma t
+
+val delete : x:int -> t:tree{is_bst t} ->
+  Tot (r:tree{is_bst r /\ not (in_tree x r)  /\
+              (forall y. x <> y ==> (in_tree y t = in_tree y r))}) (decreases t)
+let rec delete x t = match t with
+  | Leaf -> Leaf
+  | Node n t1 t2 -> if n = x then
+                      match t1, t2 with
+                      | Leaf, Leaf -> Leaf
+                      | _   , Leaf -> t1
+                      | Leaf, _    -> t2
+                      | _           -> let y = find_max t1 in
+                                       Node y (delete y t1) t2
+                    else if x < n then Node n (delete x t1) t2
+                                  else Node n t1 (delete x t2)
+
+val delete' : x : int -> t:tree -> Tot tree (decreases t)
+let rec delete' x t = match t with
+  | Leaf -> Leaf
+  | Node n t1 t2 -> if n = x then match (t1, t2) with
+                      | (Leaf, Leaf) -> Leaf
+                      | (_, Leaf) -> t1
+                      | (Leaf, _) -> t2
+                      | _ ->
+                          let y = find_max' t1 in
+                            Node y (delete' y t1) t2
+                    else if x < n then Node n (delete' x t1) t2
+                         else Node n t1 (delete' x t2)
+
+val delete_lemma : x:int -> t:tree{is_bst t} ->
+      Lemma (is_bst (delete' x t) /\ not (in_tree x (delete' x t)) /\
+        (forall y. x <> y ==> (in_tree y (delete' x t) = in_tree y t)))
+      (decreases t)
+let rec delete_lemma x t = match t with
+  | Leaf -> ()
+  | Node n t1 t2 ->
+     if x <> n then (delete_lemma x t1; delete_lemma x t2)
+     else if is_Node t1 then (find_max_lemma t1; delete_lemma (find_max' t1) t1)
